pulse/lib/steel/pulse/Pulse.Extract.CompilerLib.fsti
@@ -47,6 +47,7 @@ val e_tag_impure : e_tag
 
 val mlty_top : mlty
 
+val normalize_for_extraction (g:uenv) (t:T.term) : Dv T.term
 val term_as_mlexpr (g:uenv) (t:T.term) : Dv (mlexpr & e_tag & mlty)
 val term_as_mlty (g:uenv) (t:T.term) : Dv mlty
 
@@ -55,3 +56,5 @@ val extend_bv (g:uenv) (np:PSB.ppname) (uniq:nat) (ty:mlty) : Dv (uenv & mlident
 val initial_core_env (g:uenv) : Pulse.Typing.Env.env
 val set_tcenv (g:uenv) (e:T.env) :  uenv
 val mlexpr_to_string (e:mlexpr) : Dv string
+open Pulse.Syntax.Base
+val sigelt_extension_data (e:T.sigelt) : option st_term
